Logic/Predicate/FirstOrder/Deduction/Meta.lean
@@ -1,0 +1,75 @@
+import Logic.Predicate.FirstOrder.Deduction.Deduction
+import Logic.Predicate.FirstOrder.Meta
+
+namespace FirstOrder
+
+namespace Meta
+open Qq
+
+inductive DeductionCode (L : Q(Language.{u})) : Type
+  | trans         : Q(SyntacticFormula $L) → DeductionCode L → DeductionCode L → DeductionCode L
+  | assumption    : DeductionCode L
+  | contradiction : Q(SyntacticFormula $L) → DeductionCode L → DeductionCode L → DeductionCode L
+  | trivial       : DeductionCode L
+  | explode       : DeductionCode L → DeductionCode L
+  | intro         : DeductionCode L → DeductionCode L
+  | mdp           : Q(SyntacticFormula $L) → DeductionCode L → DeductionCode L → DeductionCode L  
+  | split         : DeductionCode L → DeductionCode L → DeductionCode L
+  -- TODO
+  | cases         : (e₁ e₂ : Q(SyntacticFormula $L)) → DeductionCode L → DeductionCode L → DeductionCode L → DeductionCode L
+  | generalize    : DeductionCode L → DeductionCode L
+  -- TODO
+  | exCases       : Q(SyntacticFormula $L) → DeductionCode L → DeductionCode L → DeductionCode L
+  | eqRefl        : DeductionCode L
+  | eqSymm        : DeductionCode L → DeductionCode L
+  | eqTrans       : Q(SyntacticFormula $L) → DeductionCode L → DeductionCode L → DeductionCode L
+  | rewriteEq     : (e₁ e₂ : Q(SyntacticTerm $L)) → DeductionCode L → DeductionCode L → DeductionCode L
+  | since         : Syntax → DeductionCode L
+  | missing       : DeductionCode L
+  -- TODO
+
+namespace DeductionCode
+variable {L : Q(Language.{u})}
+
+def toStr : DeductionCode L → String
+  | trans _ c₁ c₂         => "have: {\n" ++ c₁.toStr ++ "\n}" ++ c₂.toStr
+  | assumption            => "assumption"
+  | contradiction _ c₁ c₂ => "contradiction: {\n" ++ c₁.toStr ++ "\n}\nand: {\n" ++ c₂.toStr ++ "\n}"    
+  | trivial               => "trivial"
+  | explode c             => "explode" ++ c.toStr
+  | intro c               => "intro\n" ++ c.toStr
+  | mdp _ c₁ c₂           => "have: {\n" ++ c₁.toStr ++ "\n}\nand: {\n" ++ c₂.toStr ++ "\n}"
+  | split c₁ c₂           => "∧ split: {\n" ++ c₁.toStr ++ "\n}\nand: {\n" ++ c₂.toStr ++ "\n}"
+  | cases _ _ c₀ c₁ c₂    => "∨ split: {\n" ++ c₀.toStr ++ "\n}\nor left: {\n" ++ c₁.toStr ++ "\n}\nor right: {\n" ++ c₂.toStr ++ "\n}"
+  | generalize c          => "generalize\n" ++ c.toStr
+  | exCases _ c₀ c₁       => "∃ cases: {\n" ++ c₀.toStr ++ "\n}\n" ++ c₁.toStr
+  | eqRefl                => "refl"
+  | eqSymm c              => "symmetry" ++ c.toStr
+  | eqTrans _ c₁ c₂       => "trans: {\n" ++ c₁.toStr ++ "\n}\n and: {\n" ++ c₂.toStr ++ "\n}"
+  | rewriteEq _ _ c₁ c₂   => "rewrite: {\n" ++ c₁.toStr ++ "\n}\n" ++ c₂.toStr
+  | since _               => "since"
+  | missing               => "?"
+
+instance : Repr (DeductionCode L) := ⟨fun b _ => b.toStr⟩
+
+instance : ToString (DeductionCode L) := ⟨toStr⟩
+
+elab "test₁" : term => do
+  let L : Q(Language.{0}) := q(Language.oring)
+  let eVerum : Q(SyntacticFormula $L) := q(⊤)
+  let eFalsum : Q(SyntacticFormula $L)  := q(⊥)
+  let l₀ : List Q(SyntacticFormula $L) := [eFalsum]
+  let l₁ : List Q(SyntacticFormula $L) := eVerum :: l₀
+  let el₀ := Qq.toQList (u := levelZero) l₀
+  let el₁ := Qq.toQList (u := levelZero) l₁
+  let eb₁ := q(Proof.trivial (l := $el₀)) -- verum el eVerum
+  let some eelem := Qq.toQListOfElem eVerum l₁ | throwError "err" --el eVerum
+  let eb₂ : Q(Proof [Formula.verum, Formula.falsum] Formula.verum) := q(Proof.assumption $eelem)
+  let eb₁₂ := q(Proof.block $eb₁ $eb₂)
+  return eb₁₂
+
+end DeductionCode
+
+end Meta
+
+end FirstOrder
